secure_api/merkle_tree/MerkleTree.New.High.Correct.Path.fst
@@ -1,0 +1,78 @@
+module MerkleTree.New.High.Correct.Path
+
+open EverCrypt
+open EverCrypt.Helpers
+
+open MerkleTree.Spec
+open MerkleTree.New.High
+open MerkleTree.New.High.Correct.Base
+
+open FStar.Classical
+open FStar.Ghost
+open FStar.Seq
+
+module List = FStar.List.Tot
+module S = FStar.Seq
+
+module U32 = FStar.UInt32
+module U8 = FStar.UInt8
+type uint32_t = U32.t
+type uint8_t = U8.t
+
+module EHS = EverCrypt.Hash
+module MTS = MerkleTree.Spec
+
+/// Correctness of path generation
+
+val path_spec:
+  k:nat ->
+  j:nat{k <= j} ->
+  actd:bool ->
+  p:path{S.length p = mt_path_length k j actd} ->
+  GTot (sp:S.seq MTS.hash{S.length sp = log2c j})
+       (decreases (S.length p))
+#reset-options "--z3rlimit 10"
+let rec path_spec k j actd p =
+  if S.length p = 0 then S.empty
+  else if j = 0 then S.empty
+  else (S.cons
+         (if k % 2 = 0
+         then (if j = k || (j = k + 1 && not actd) 
+              then HPad else HRaw (S.head p))
+         else HRaw (S.head p))
+         (path_spec (k / 2) (j / 2) (actd || (j % 2 = 1)) (S.tail p)))
+#reset-options
+
+// val mt_get_path_acc:
+//   i:nat -> 
+//   j:nat{i <= j} ->
+//     hs_wf_elts lv hs i j} ->
+//   hs:hash_ss{S.length hs = 32} ->
+//   rhs:hash_seq{S.length rhs = 32} ->
+//   k:nat{i <= k && k <= j} ->
+//   p:path ->
+//   actd:bool ->
+//   GTot (np:path{S.length np = S.length p + mt_path_length k j actd})
+//        (decreases (32 - lv))
+
+// #reset-options "--z3rlimit 10"
+// val mt_get_path_sim:
+//   lv:nat{lv <= 32} ->
+//   i:nat -> 
+//   j:nat{i <= j /\ j < pow2 (32 - lv)} ->
+//   olds:hash_ss{S.length olds = 32 /\ mt_olds_inv lv i olds} ->
+//   hs:hash_ss{S.length hs = 32 /\ hs_wf_elts lv hs i j} ->
+//   rhs:hash_seq{S.length rhs = 32} ->
+//   k:nat{i <= k && k <= j} ->
+//   p:path ->
+//   actd:bool ->
+//   Lemma (requires (j > 0))
+//         (ensures (mt_olds_hs_lth_inv_ok lv i j olds hs;
+//                  S.equal (path_spec k j actd
+//                            (S.slice (mt_get_path_ lv hs rhs i j k p actd)
+//                            (S.length p) (S.length p + mt_path_length k j actd)))
+//                          (MTS.mt_get_path #(log2c j)
+//                            (hash_seq_spec (S.index (merge_hs olds hs) lv)) k)))
+//         (decreases j)
+  
+
